dev/lf/mutation-tight-proof/General_to_tight.v
@@ -12,13 +12,13 @@ Require Import Tight_possible_types.
 (** ** Tight to precise *)
 
 (* Lemma 1 *)
-Lemma tight_to_precise_typ_dec: forall G x A S U,
+Lemma tight_to_precise_typ_dec: forall G S x A V U,
   inert G ->
-  ty_trm ty_general sub_tight G (trm_var (avar_f x)) (typ_rcd (dec_typ A S U)) ->
+  ty_trm ty_general sub_tight G S (trm_var (avar_f x)) (typ_rcd (dec_typ A V U)) ->
   exists T,
-    ty_trm ty_precise sub_general G (trm_var (avar_f x)) (typ_rcd (dec_typ A T T)) /\
-    subtyp ty_general sub_tight G T U /\
-    subtyp ty_general sub_tight G S T.
+    ty_trm ty_precise sub_general G S (trm_var (avar_f x)) (typ_rcd (dec_typ A T T)) /\
+    subtyp ty_general sub_tight G S T U /\
+    subtyp ty_general sub_tight G S V T.
 Proof.
   introv HG Ht.
   lets Htp: (tight_possible_types_lemma HG Ht). clear Ht.
@@ -26,16 +26,16 @@ Proof.
   - lets Hp: (inert_precise_dec_typ_inv HG H). subst.
     exists U. split*.
   - specialize (IHHtp A T U0 HG eq_refl).
-    destruct IHHtp as [V [Hx [Hs1 Hs2]]].
-    exists V. split*.
+    destruct IHHtp as [W [Hx [Hs1 Hs2]]].
+    exists W. split*.
 Qed.
 
-Lemma tight_to_precise_trm_dec: forall G x a T,
+Lemma tight_to_precise_trm_dec: forall G S x a T,
   inert G ->
-  ty_trm ty_general sub_tight G (trm_var (avar_f x)) (typ_rcd (dec_trm a T)) ->
+  ty_trm ty_general sub_tight G S (trm_var (avar_f x)) (typ_rcd (dec_trm a T)) ->
   exists T',
-    ty_trm ty_precise sub_general G (trm_var (avar_f x)) (typ_rcd (dec_trm a T')) /\
-    subtyp ty_general sub_tight G T' T.
+    ty_trm ty_precise sub_general G S (trm_var (avar_f x)) (typ_rcd (dec_trm a T')) /\
+    subtyp ty_general sub_tight G S T' T.
 Proof.
   introv Hgd Ht.
   lets Htp: (tight_possible_types_lemma Hgd Ht). clear Ht.
@@ -46,43 +46,43 @@ Proof.
     eapply subtyp_trans; eassumption.
 Qed.
 
-Lemma tight_to_precise_typ_all: forall G x S T,
+Lemma tight_to_precise_typ_all: forall G S x V T,
   inert G ->
-  ty_trm ty_general sub_tight G (trm_var (avar_f x)) (typ_all S T) ->
-  exists S' T' L,
-    ty_trm ty_precise sub_general G (trm_var (avar_f x)) (typ_all S' T') /\
-    subtyp ty_general sub_tight G S S' /\
+  ty_trm ty_general sub_tight G S (trm_var (avar_f x)) (typ_all V T) ->
+  exists V' T' L,
+    ty_trm ty_precise sub_general G S (trm_var (avar_f x)) (typ_all V' T') /\
+    subtyp ty_general sub_tight G S V V' /\
     (forall y,
         y \notin L ->
-            subtyp ty_general sub_general (G & y ~ S) (open_typ y T') (open_typ y T))
+            subtyp ty_general sub_general (G & y ~ V) S (open_typ y T') (open_typ y T))
     .
 Proof.
   introv HG Ht.
   lets Htp: (tight_possible_types_lemma HG Ht). clear Ht.
   dependent induction Htp.
-  - exists S T (dom G); auto.
+  - exists V T (dom G); auto.
   - specialize (IHHtp _ _ HG eq_refl).
-    destruct IHHtp as [S' [T' [L' [Hpt [HSsub HTsub]]]]].
-    exists S' T' (dom G \u L \u L').
+    destruct IHHtp as [V' [T' [L' [Hpt [HSsub HTsub]]]]].
+    exists V' T' (dom G \u L \u L').
     split; auto.
-    assert (Hsub2 : subtyp ty_general sub_tight G (typ_all S0 T0) (typ_all S T)).
+    assert (Hsub2 : subtyp ty_general sub_tight G S (typ_all V0 T0) (typ_all V T)).
     { apply subtyp_all with (L:=L); assumption. }
     split.
     + eapply subtyp_trans; eauto.
     + intros y Fr.
-      assert (Hok: ok (G & y ~ S)) by auto using ok_push, inert_ok.
+      assert (Hok: ok (G & y ~ V)) by auto using ok_push, inert_ok.
       apply tight_to_general in H; auto.
-      assert (Hnarrow: subtyp ty_general sub_general (G & y ~ S) (open_typ y T') (open_typ y T0)).
+      assert (Hnarrow: subtyp ty_general sub_general (G & y ~ V) S (open_typ y T') (open_typ y T0)).
       { eapply narrow_subtyping; auto using subenv_last. }
       eauto.
 Qed.
 
 (* Lemma 2 *)
-Lemma tight_subtyping_sel: forall G x A S U,
+Lemma tight_subtyping_sel: forall G S x A V U,
     inert G ->
-    ty_trm ty_general sub_tight G (trm_var (avar_f x)) (typ_rcd (dec_typ A S U)) ->
-    (subtyp ty_general sub_tight G (typ_sel (avar_f x) A) U /\
-     subtyp ty_general sub_tight G S (typ_sel (avar_f x) A)).
+    ty_trm ty_general sub_tight G S (trm_var (avar_f x)) (typ_rcd (dec_typ A V U)) ->
+    (subtyp ty_general sub_tight G S (typ_sel (avar_f x) A) U /\
+     subtyp ty_general sub_tight G S V (typ_sel (avar_f x) A)).
 Proof.
   introv HG Hty.
   pose proof (tight_to_precise_typ_dec HG Hty) as [T [Ht [Hs1 Hs2]]].
@@ -94,27 +94,27 @@ Qed.
 (* Theorem 1 *)
 Lemma general_to_tight: forall G0,
   inert G0 ->
-  (forall m1 m2 G t T,
-     ty_trm m1 m2 G t T ->
+  (forall m1 m2 G S t T,
+     ty_trm m1 m2 G S t T ->
      G = G0 ->
      m1 = ty_general ->
      m2 = sub_general ->
-     ty_trm ty_general sub_tight G t T) /\
-  (forall m1 m2 G S U,
-     subtyp m1 m2 G S U ->
+     ty_trm ty_general sub_tight G S t T) /\
+  (forall m1 m2 G S V U,
+     subtyp m1 m2 G S V U ->
      G = G0 ->
      m1 = ty_general ->
      m2 = sub_general ->
-     subtyp ty_general sub_tight G S U).
+     subtyp ty_general sub_tight G S V U).
 Proof.
   intros G0 HG.
   apply ts_mutind; intros; subst; try solve [eapply tight_subtyping_sel; auto]; eauto.
 Qed.
 
-Lemma general_to_tight_typing: forall G t T,
+Lemma general_to_tight_typing: forall G S t T,
   inert G ->
-  ty_trm ty_general sub_general G t T ->
-  ty_trm ty_general sub_tight G t T.
+  ty_trm ty_general sub_general G S t T ->
+  ty_trm ty_general sub_tight G S t T.
 Proof.
   intros. apply* general_to_tight.
 Qed.
